src/lowparse/LowParse.Spec.Option.fst
@@ -8,6 +8,7 @@ module U32 = FStar.UInt32
 let parse_option_kind (k: parser_kind) : Tot parser_kind = {
   parser_kind_metadata = {
     parser_kind_metadata_total = false;
+    parser_kind_metadata_fail = false;
   };
   parser_kind_low = 0;
   parser_kind_high = k.parser_kind_high;
